Semantics/Imp/Structural.lean
@@ -5,85 +5,85 @@ namespace Com
 namespace Structural
 
 inductive step: Com × State → Com × State → Prop where
-  | ass:
-    step (x = a, s) (skip, s⟪x ≔ a⇓s⟫)
+  | assₛ:
+    step (x = a, s) (skip₁, s⟪x ≔ a⇓s⟫)
 
-  | cat_skip:
-    step (skip;;c, s) (c, s)
+  | cat₀ₛ:
+    step (skip₁;;c, s) (c, s)
 
-  | cat_step (h: step (c, s) (e, t)):
+  | catₙₛ (h: step (c, s) (e, t)):
     step (c;;d, s) (e;;d, t)
 
-  | cond:
+  | ifₛ:
     step (if b then c else d end, s) (bif b⇓s then c else d, s)
 
-  | loop:
-    step (while b loop c end, s) (bif b⇓s then c;;while b loop c end else skip, s)
+  | whileₛ:
+    step (while b loop c end, s) (bif b⇓s then c;;while b loop c end else skip₁, s)
 
 infix:110 " ⇒ " => step
 
 private example:
-  (⦃x = 0; while x <= 2 {x = x + 1}⦄, σ₀) ⇒
-      (⦃skip; while x <= 2 {x = x + 1}⦄, σ₀⟪"x" ≔ 0⟫) := step.cat_step step.ass
+  (⦃x = 0; while x <= 2 loop x = x + 1 end⦄, σ₀) ⇒
+      (⦃skip; while x <= 2 loop x = x + 1 end⦄, σ₀⟪"x" ≔ 0⟫) :=
+  step.catₙₛ step.assₛ
 
 theorem cat_iff:
   (c₁;;c₂, s) ⇒ et
     ↔ (∃e t, (c₁, s) ⇒ (e, t) ∧ et = (e;;c₂, t))
-      ∨ (c₁ = skip ∧ et = (c₂, s)) := by
-  constructor <;> intro h
-  . cases h with
-    | cat_skip => exact Or.inr ⟨rfl, rfl⟩
-    | cat_step h => exact Or.inl ⟨_, ⟨_, ⟨h, rfl⟩⟩⟩
-  . cases h with
-    | inl h =>
-      cases h with
-      | intro e h =>
-        cases h with
-        | intro t h =>
-          exact h.right ▸ step.cat_step h.1
-    | inr h =>
-      cases h with
-      | intro h1 h2 =>
-        exact h1 ▸ h2 ▸ step.cat_skip
+      ∨ (c₁ = skip₁ ∧ et = (c₂, s)) :=
+  ⟨fun h =>
+    match h with
+    | step.cat₀ₛ => Or.inr ⟨rfl, rfl⟩
+    | step.catₙₛ h => Or.inl ⟨_, ⟨_, ⟨h, rfl⟩⟩⟩,
+    fun h => match h with
+    | Or.inl h => match h with
+      | Exists.intro _ h => match h with
+        | Exists.intro _ h => h.2 ▸ step.catₙₛ h.1
+    | Or.inr h => match h with
+      | And.intro h1 h2 => h1 ▸ h2 ▸ step.cat₀ₛ⟩
 
 theorem cond_iff:
   (if b then c else d end, s) ⇒ ss
-    ↔ (b⇓s ∧ ss = (c, s)) ∨ (b⇓s = false ∧ ss = (d, s)) := by
-  constructor <;> intro h
-  . cases hb: b⇓s <;> cases h
-    . exact Or.inr ⟨rfl, hb ▸ rfl⟩
-    . exact Or.inl ⟨rfl, hb ▸ rfl⟩
-  . have hss: ss = (bif b⇓s then c else d, s) := by
-      cases hb: b⇓s <;> rw [hb] at h <;> simp at * <;> assumption
-    exact hss ▸ step.cond
+    ↔ (b⇓s ∧ ss = (c, s)) ∨ (b⇓s = false ∧ ss = (d, s)) :=
+  ⟨fun h => match hb: b⇓s with
+    | false => match h with | step.ifₛ => Or.inr ⟨rfl, hb ▸ rfl⟩
+    | true => match h with | step.ifₛ => Or.inl ⟨rfl, hb ▸ rfl⟩,
+    fun h =>
+      let hss: ss = (bif b⇓s then c else d, s) :=
+        match hb: b⇓s with
+        | true => match hb ▸ h with | Or.inl h => h.2
+        | false => match hb ▸ h with | Or.inr h => h.2
+      hss ▸ step.ifₛ⟩
 
 theorem cond_false {b: Bexp} (hb: b⇓s = false):
-  (if b then c else d end, s) ⇒ ss ↔ (ss = (d, s)) :=
-  by
-    simp [cond_iff, hb]
+  (if b then c else d end, s) ⇒ ss ↔ (ss = (d, s)) := by
+  rw [cond_iff, hb]
+  exact ⟨fun h => match h with
+    | Or.inr h => match h with | And.intro _ h2 => h2,
+    fun h => Or.inr ⟨rfl, h⟩⟩
 
 infix:110 " ⇒* " => RTL step
 
 theorem star.demo₂:
-  (⦃x = 2; while 0 <= x {x = x + 1}⦄, σ₀) ⇒*
-      (⦃while 0 <= x {x = x + 1}⦄, σ₀⟪"x" ≔ 2⟫) :=
-  RTL.head (step.cat_step step.ass) (RTL.head step.cat_skip RTL.refl)
+  (⦃x = 2; while 0 <= x loop x = x + 1 end⦄, σ₀) ⇒*
+      (⦃while 0 <= x loop x = x + 1 end⦄, σ₀⟪"x" ≔ 2⟫) :=
+  RTL.head (step.catₙₛ step.assₛ) (RTL.head step.cat₀ₛ RTL.refl)
 
 theorem star.cat_skip_cat
   (h: (c, s) ⇒* (skip, t)):
   (c;;d, s) ⇒* (skip;;d, t) :=
-  RTL.lift (fun (x: Com × State) => (x.1;;d, x.2)) (fun _ _ h => step.cat_step h) h
+  RTL.lift (fun (x: Com × State) => (x.1;;d, x.2)) (fun _ _ h => step.catₙₛ h) h
 
 theorem star.cat
-  (h1: (c₁, s) ⇒* (skip, s₁))
-  (h2: (c₂, s₁) ⇒* (skip, s₂)):
-  (c₁;;c₂, s) ⇒* (skip, s₂) :=
-  RTL.trans (cat_skip_cat h1) (RTL.trans (RTL.single step.cat_skip) h2)
+  (h1: (c₁, s) ⇒* (skip₁, s₁))
+  (h2: (c₂, s₁) ⇒* (skip₁, s₂)):
+  (c₁;;c₂, s) ⇒* (skip₁, s₂) :=
+  RTL.trans (cat_skip_cat h1) (RTL.trans (RTL.single step.cat₀ₛ) h2)
 
 theorem star.cat_no_influence
-  (h: (c₁, s) ⇒* (skip, s₁)):
+  (h: (c₁, s) ⇒* (skip₁, s₁)):
   (c₁;;c₂, s) ⇒* (c₂, s₁) :=
-  RTL.trans (cat_skip_cat h) (RTL.single step.cat_skip)
+  RTL.trans (cat_skip_cat h) (RTL.single step.cat₀ₛ)
 
 end Structural
 end Com
