Semantics/Imp/Equivalence.lean
@@ -4,42 +4,48 @@ import Semantics.Imp.Denotational
 
 namespace Com
 
-theorem Structural.from_natural {c: Com} (h: w ⊢ c ⟹ s): (c, w) ⇒* (skip, s) := by
+theorem Structural.from_natural {c: Com}
+  (h: w ⊢ c ⟹ s): (c, w) ⇒* (skip₁, s) := by
   induction h with
-  | skip => exact RTL.refl
-  | ass => exact RTL.single step.ass
-  | cat _ _ _ ihc ihd => exact star.cat ihc ihd
-  | cond_true hb _ ih => exact RTL.head step.cond (hb ▸ ih)
-  | cond_false hb _ ih => exact RTL.head step.cond (hb ▸ ih)
-  | loop_true _ hb _ _ ihc ihw =>
-    exact RTL.head step.loop $ RTL.trans (hb ▸ star.cat ihc ihw) RTL.refl
-  | loop_false hb =>
-    exact RTL.head step.loop $ hb ▸ RTL.refl
+  | skipₙ => exact RTL.refl
+  | assₙ => exact RTL.single step.assₛ
+  | catₙ _ _ _ ihc ihd => exact star.cat ihc ihd
+  | if₁ₙ hb _ ih => exact RTL.head step.ifₛ (hb ▸ ih)
+  | if₀ₙ hb _ ih => exact RTL.head step.ifₛ (hb ▸ ih)
+  | while₁ₙ _ hb _ _ ihc ihw =>
+    exact RTL.head step.whileₛ $ RTL.trans (hb ▸ star.cat ihc ihw) RTL.refl
+  | while₀ₙ hb =>
+    exact RTL.head step.whileₛ $ hb ▸ RTL.refl
 
-theorem Natural.from_structural_step (h₁: x ⇒ y) (h₂: y.2 ⊢ y.1  ⟹ s): x.2 ⊢ x.1 ⟹ s := by
+theorem Natural.from_structural_step
+  (h₁: x ⇒ y) (h₂: y.2 ⊢ y.1  ⟹ s): x.2 ⊢ x.1 ⟹ s := by
   induction h₁ generalizing s with
-  | ass => exact (skip_iff.mp h₂) ▸ step.ass
-  | cat_skip => exact step.cat _ step.skip h₂
-  | cat_step _ ih =>
-    cases h₂ with
-    | cat w hc hd => exact step.cat w (ih hc) hd
-  | cond => rw [cond_iff']; exact h₂
-  | _ => rw [loop_unfold, cond_iff']; exact h₂
+  | assₛ => exact (skip_iff.mp h₂) ▸ step.assₙ
+  | cat₀ₛ => exact step.catₙ _ step.skipₙ h₂
+  | catₙₛ _ ih =>
+    match h₂ with
+    | step.catₙ w hc hd => exact step.catₙ w (ih hc) hd
+  | ifₛ => rw [if_iff']; exact h₂
+  | whileₛ => rw [loop_unfold, if_iff']; exact h₂
 
-theorem Natural.from_structural (h: x ⇒* (skip, t)): x.2 ⊢ x.1 ⟹ t := by
+theorem Natural.from_structural
+  (h: x ⇒* (skip₁, t)): x.2 ⊢ x.1 ⟹ t := by
   induction h using RTL.head_induction_on with
-  | refl => exact step.skip
+  | refl => exact step.skipₙ
   | head h _ ht => exact from_structural_step h ht
 
-theorem structural_iff_natural: (c, s) ⇒* (skip, t) ↔ (s ⊢ c ⟹ t) := ⟨Natural.from_structural, Structural.from_natural⟩
+theorem structural_iff_natural:
+  (c, s) ⇒* (skip₁, t) ↔ (s ⊢ c ⟹ t) :=
+  ⟨Natural.from_structural, Structural.from_natural⟩
 
-theorem denote.from_natural {c: Com} (h: s ⊢ c ⟹ t): (s, t) ∈ ⟦c⟧ := by
+theorem denote.from_natural {c: Com}
+  (h: s ⊢ c ⟹ t): (s, t) ∈ ⟦c⟧ := by
   induction h with
-  | skip => exact SRel.mem_id.mpr rfl
-  | ass  => exact SRel.mem_id.mpr rfl
-  | cat t _ _ ih₁ ih₂ => exact ⟨t, ⟨ih₁, ih₂⟩⟩
-  | cond_true hb _ ih => exact Or.inl ⟨ih, hb⟩
-  | cond_false hb _ ih =>
+  | skipₙ => exact SRel.mem_id.mpr rfl
+  | assₙ  => exact SRel.mem_id.mpr rfl
+  | catₙ t _ _ ih₁ ih₂ => exact ⟨t, ⟨ih₁, ih₂⟩⟩
+  | if₁ₙ hb _ ih => exact Or.inl ⟨ih, hb⟩
+  | if₀ₙ hb _ ih =>
       apply Or.inr
       rw [
         Set.mem_diff,
@@ -50,9 +56,10 @@ theorem denote.from_natural {c: Com} (h: s ⊢ c ⟹ t): (s, t) ∈ ⟦c⟧ := b
         and_true
       ]
       exact ih
-  | loop_true t hb _ _ ih₁ ih₂ => exact loop_unfold ▸ Or.inl ⟨⟨t, ⟨ih₁, ih₂⟩⟩, hb⟩
-  | loop_false hb =>
-      rw [loop_unfold]
+  | while₁ₙ t hb _ _ ih₁ ih₂ =>
+    exact while_unfold ▸ Or.inl ⟨⟨t, ⟨ih₁, ih₂⟩⟩, hb⟩
+  | while₀ₙ hb =>
+      rw [while_unfold]
       apply Or.inr
       rw [
         Set.mem_diff,
@@ -67,42 +74,55 @@ theorem denote.from_natural {c: Com} (h: s ⊢ c ⟹ t): (s, t) ∈ ⟦c⟧ := b
 theorem Natural.from_denote (h: (s, t) ∈ ⟦c⟧): s ⊢ c ⟹ t := by
   revert h
   induction c generalizing s t with
-  | skip => intro h; cases h; exact step.skip
-  | ass =>
+  | skip₁ =>
+    intro h
+    rw [denote, SRel.mem_id] at h
+    exact h ▸ step.skipₙ
+  | ass₁ =>
     intro h
     rw [denote.eq_def, Set.mem_comprehend] at h
     simp at h
-    exact h ▸ step.ass
-  | cat _ _ ih₁ ih₂ =>
+    exact h ▸ step.assₙ
+  | cat₁ _ _ ih₁ ih₂ =>
     intro h
-    cases h with | intro w h =>
-      exact step.cat w (ih₁ h.left) (ih₂ h.right)
-  | cond _ _ _ ih₁ ih₂ =>
+    match h with
+    | Exists.intro w h =>
+      exact step.catₙ w (ih₁ h.left) (ih₂ h.right)
+  | if₁ _ _ _ ih₁ ih₂ =>
     intro h
-    cases h with
-    | inl h =>
-      cases h with | intro h hb =>
-        exact step.cond_true hb (ih₁ h)
-    | inr h =>
-      cases h with | intro h hb =>
+    match h with
+    | Or.inl h =>
+      match h with
+      | And.intro h hb =>
+        exact step.if₁ₙ hb (ih₁ h)
+    | Or.inr h =>
+      match h with
+      | And.intro h hb =>
         simp [Set.mem_comprehend] at hb
-        exact step.cond_false hb (ih₂ h)
-  | _ b c ih =>
-    suffices ⟦while b loop c end⟧ ⊆ {s | s.1 ⊢ while b loop c end ⟹ s.2} by apply this
+        exact step.if₀ₙ hb (ih₂ h)
+  | while₁ b c ih =>
+    suffices
+      ⟦while b loop c end⟧ ⊆ {s | s.1 ⊢ while b loop c end ⟹ s.2} by
+      apply this
     apply Fix.lfp_le
     intro ss h
-    cases ss with | mk =>
-      cases h with
-      | inl h =>
-        cases h with | intro h hb =>
-          cases h with | intro w h =>
-            exact step.loop_true w hb (ih h.left) h.right
-      | inr h =>
-        cases h with | intro hq hb =>
+    match ss with
+    | Prod.mk _ _ =>
+      match h with
+      | Or.inl h =>
+        match h with
+        | And.intro h hb =>
+          match h with
+          | Exists.intro w h =>
+            exact step.while₁ₙ w hb (ih h.left) h.right
+      | Or.inr h =>
+        match h with
+        | And.intro hq hb =>
           simp [Set.mem_comprehend] at hb
           rw [SRel.mem_id] at hq
-          exact hq ▸ step.loop_false hb
+          exact hq ▸ step.while₀ₙ hb
 
-theorem natural_iff_denote: (s, t) ∈ ⟦c⟧ ↔ (s ⊢ c ⟹ t) := ⟨Natural.from_denote, denote.from_natural⟩
+theorem natural_iff_denote: (s, t) ∈ ⟦c⟧ ↔ (s ⊢ c ⟹ t) :=
+  ⟨Natural.from_denote, denote.from_natural⟩
 
 end Com
